AP/Util/Data/Trie.lean
@@ -1,11 +1,18 @@
 import AP.Util.Data.Set
 
+namespace Trie
+
 open Std
 
-inductive TrieRaw (α β : Type*) [DecidableEq α] [Hashable α] where
-| mk : Option β → DHashMap.Raw α (λ _ => TrieRaw α β) → TrieRaw α β
+inductive Raw (α β : Type*) [DecidableEq α] [Hashable α] where
+| mk : Option β → DHashMap.Raw α (λ _ => Raw α β) → Raw α β
 
 variable {α β : Type*} [ha₁ : DecidableEq α] [ha₂ : Hashable α]
+
+-- def Raw.rec' {γ : Sort*}
+-- (motive : ∀ (val : Option β) (mp : DHashMap.Raw α (λ _ => Raw α β)),
+-- (∀ i x, mp.get? i = some x → γ) → γ) : (raw : Raw α β) → γ
+-- | .mk val mp => motive val mp # λ g => mp.foldlWith _ _ _
 
 -- def TrieRaw.depth : TrieRaw α β → ℕ
 -- | mk _ mp => mp.fold (λ acc _ trie => max acc # 1 + trie.depth) 0
